$$
sin(A + B) = sinAcosB + cosAsinB \\
sin(A - B) = sinAcosB - cosAsinB \\
cos(A + B) = cosAcosB - sinAsinB \\
cos(A - B) = cosAcosB + sinAsinB \\
tan(A + B) = \frac{tanA + tanB}{1 - tanAtanB} \\
tan(A - B) = \frac{tanA - tanB}{1 + tanAtanB} \\
cot(A + B) = \frac{cotAcotB - 1}{cotB + cotA} \\
cot(A - B) = \frac{cotAcotB + 1}{cotB - cotA} \\
\\
tan2A = \frac{2tanA}{1 - tan^2A} \\
sin2A = 2sinAcosA \\
cos2A = 2cos^2A - 1 = 1 - 2sin^2A \\
\\
sin3A = 3sinA - 4sin^3A \\
cos3A = 4cos^3A - 3cosA \\
tan3A = tanA tan(\frac{\pi}{3} + A) tan(\frac{\pi}{3} - A) \\
\\
sinA + sinB = 2sin\frac{a + b}{2}cos\frac{a - b}{2} \\
sinA - sinB = 2cos\frac{a + b}{2}sin\frac{a - b}{2} \\
cosA + cosB = 2cos\frac{a + b}{2}cos\frac{a - b}{2} \\
cosA - cosB = -2sin\frac{a + b}{2}sin\frac{a - b}{2} \\
tanA + tanB = \frac{sin(A + B)}{cosAcosB} \\
\\
sinAsinB = -\frac{1}{2}[cos(a + b) - cos(a - b)] \\
cosAcosB = \frac{1}{2}[cos(a + b) + cos(a - b)] \\
sinAcosB = \frac{1}{2}[sin(A + B) + sin(A - B)] \\
cosAsinB = \frac{1}{2}[sin(A + B) - sin(A - B)] \\
\\
sin(-A) = -sinA \\
cos(-A) = cosA \\
sin(\frac{\pi}{2} - A) = cosA \\
cos(\frac{\pi}{2} - A) = sinA \\
sin(\frac{\pi}{2} + A) = cosA \\
cos(\frac{\pi}{2} + A) = -sinA \\
sin(\pi - A) = sinA \\
cos(\pi - A) = -cosA \\
sin(\pi + A) = -sinA \\
cos(\pi + A) = -cosA \\
tan(\pi + A) = tanA \\
cot(\pi + A) = cotA \\
\\
sinA = \frac{2tan\frac{A}{2}}{1 + tan^2\frac{A}{2}} \\
cosA = \frac{1 - tan^2\frac{A}{2}}{1 + tan^2\frac{A}{2}} \\
tanA = \frac{2tan\frac{A}{2}}{1 - tan^2\frac{A}{2}} \\
\\
asinA + bcosA = \sqrt{a^2 + b^2}sin(A + B) \ (tanB = \frac{b}{a}) \\
asinA - bcosA = \sqrt{a^2 + b^2}cos(A - B) \ (tanB = \frac{a}{b}) \\
\\
arctanx = arccot\frac{1}{x} \\
arccotx = arctan\frac{1}{x} \\
arsinx + arccosx = \frac{\pi}{2} \\
$$

